proof/Anomaly.thy
@@ -1,5 +1,5 @@
 theory Anomaly
-  imports Main DSG
+  imports Main DSG Observation
 begin
 
 section \<open>Non-Cyclic Anomalies\<close>
@@ -38,6 +38,35 @@ text \<open>In an G0 anomaly, a cycle exists in the DSG composed purely of write
 definition has_g0 :: "history \<Rightarrow> bool" where
 "has_g0 h \<equiv> (\<exists>path. (cycle (dsg h) path) \<and> ((path_dep_types path) = {WW}))"
 
+text \<open>For example...\<close>
+
+lemma ww_depends_ex:
+  assumes "(distinct [x,y]) \<and> (distinct [v0,v1,v2])"
+  shows "ww_depends (History objs
+                         {(ATxn [(AWrite x v0 a1 v1 r1), (AWrite y v1 a2 v2 r2)] True),
+                          (ATxn [(AWrite y v0 a1 v1 r1), (AWrite x v1 a2 v2 r2)] True)}
+                         {(KeyVersionOrder x [v0,v1,v2]),
+                          (KeyVersionOrder y [v0,v1,v2])})
+                      (ATxn [(AWrite x v0 a1 v1 r1), (AWrite y v1 a2 v2 r2)] True)
+                      (ATxn [(AWrite y v0 a1 v1 r1), (AWrite x v1 a2 v2 r2)] True)"
+  apply (simp add:ww_depends_def)
+proof-
+  obtain t1 t2 where "t1 = (ATxn [(AWrite x v0 a1 v1 r1), (AWrite y v1 a2 v2 r2)] True) \<and>
+                      t2 = (ATxn [(AWrite y v0 a1 v1 r1), (AWrite x v1 a2 v2 r2)] True)"
+    by blast
+  oops
+
+
+lemma
+  assumes "(distinct [x,y]) \<and> (distinct [v0,v1,v2])"
+  shows "has_g0 (History objs
+                         {(ATxn [(AWrite x v0 a1 v1 r1), (AWrite y v1 a2 v2 r2)] True),
+                          (ATxn [(AWrite y v0 a1 v1 r1), (AWrite x v1 a2 v2 r2)] True)}
+                         {(KeyVersionOrder x [v0,v1,v2]),
+                          (KeyVersionOrder y [v0,v1,v2])})"
+  apply (simp add:has_g0_def dsg_def path_def cycle_def)
+  oops
+
 text \<open>A G1c anomaly is a cycle comprised of write-write and write-read dependencies. We diverge from
 Adya here in classifying G0 and G1c as distinct classes; feels more useful to distinguish them.\<close>
 
@@ -48,3 +77,7 @@ text \<open>And a G2 anomaly is a cycle involving read-write dependencies.\<clos
 
 definition has_g2 :: "history \<Rightarrow> bool" where
 "has_g2 h \<equiv> (\<exists>path. (cycle (dsg h) path) \<and> (RW \<in> (path_dep_types path)))"
+
+
+
+end
