proof/IDSG.thy
@@ -1,0 +1,39 @@
+theory IDSG
+  imports Main Observation
+begin
+
+section \<open>Inferred Version Order\<close>
+
+text \<open>We begin by inferring a version order based on traceability and recoverability. TODO: we're
+not handling intermediate dependencies yet.\<close>
+
+text \<open>Pick a version from the committed read set with the longest trace.\<close>
+
+value "((\<lambda>x::nat. (Suc x)) ` ({1,2}))"
+
+definition o_committed_txns :: "observation \<Rightarrow> otxn set" where
+"o_committed_txns obs \<equiv> {t \<in> (all_otxns obs). o_definitely_committed t}"
+
+definition o_committed_reads :: "observation \<Rightarrow> oop set" where
+"o_committed_reads obs \<equiv> \<Union>(all_oreads ` (o_committed_txns obs))"
+
+definition o_committed_versions_k :: "observation \<Rightarrow> key \<Rightarrow> version set" where
+"o_committed_versions_k obs k \<equiv>
+  \<Union>(all_versions ` {r. r \<in> (o_committed_reads obs) \<and> ((key r) = k)})"
+
+definition x_longest :: "observation \<Rightarrow> k \<Rightarrow> version"
+"x_longest obs \<equiv> (let vs (o_committed_versions obs k) in
+                    (THE v. (v \<in> vs) \<and> \<not>(\<exists>v2. (trace_length v1) < (trace_length v2))
+
+TODO what a mess; pick up here later
+
+section \<open>Inferred Transaction Dependencies\<close>
+
+
+
+text \<open>We use recoverability to map observed versions in a history back into writes, and infer
+dependencies between them.\<close>
+
+definition 
+
+end
