proof/Observation.thy
@@ -1,0 +1,140 @@
+theory Observation
+  imports Main History
+begin
+
+section \<open>Observations\<close>
+
+text \<open>Fundamentally, an observation is a set of objects and observed transactions over them.\<close>
+
+datatype observation = Observation "object set" "otxn set"
+
+text \<open>We define some basic accessors...\<close>
+
+primrec all_otxns :: "observation \<Rightarrow> otxn set" where
+"all_otxns (Observation objs txns) = txns"
+
+instantiation observation :: all_objects
+begin
+primrec all_objects_observation :: "observation \<Rightarrow> object set" where
+"all_objects_observation (Observation objs txns) = objs"
+instance ..
+end
+
+instantiation observation :: all_versions
+begin
+primrec all_versions_observation :: "observation \<Rightarrow> version set" where
+"all_versions_observation (Observation objs txns) = \<Union>{all_versions t | t. t \<in> txns}"
+instance ..
+end
+
+instantiation observation :: all_oops
+begin
+primrec all_oops_observation :: "observation \<Rightarrow> oop set" where
+"all_oops_observation (Observation objs txns) = \<Union>{all_oops t | t. t \<in> txns}"
+instance ..
+end
+
+text \<open>A well-formed observation is made up of well-formed objects and transactions, and its
+transactions are over those objects.\<close>
+
+primrec wf_observation :: "observation \<Rightarrow> bool" where
+"wf_observation (Observation objs txns) =
+  ((\<forall>obj. obj \<in> objs \<longrightarrow> wf_object obj) \<and>
+   (\<forall>t. t \<in> txns \<longrightarrow> (wf_otxn t \<and> (\<forall>oop. (oop \<in> (all_oops t)) \<longrightarrow>
+                                          (\<exists>!obj. (obj \<in> objs) \<and> ((key oop) = (key obj)))))))"
+
+
+text \<open>We say an observation is compatible with a history via relation m if they have the same
+object set, the same number of transactions, and m is a bijective mapping from observed transactions
+in the observation to compatible abstract transactions in the history.\<close>
+
+definition is_compatible_observation :: "observation \<Rightarrow> (otxn \<Rightarrow> atxn) \<Rightarrow> history \<Rightarrow> bool" where
+"is_compatible_observation obs m h =
+  ((all_objects obs = all_objects h) \<and>
+   (\<forall>otxn. otxn \<in> (all_otxns obs) \<longrightarrow> (is_compatible_txn otxn (m otxn))))"
+
+
+section \<open>Interpretations\<close>
+
+text \<open>An interpretation of an observation O is a history H and a bijection M which translates
+operations in O to compatible observations in H. Interpretation is a reserved word, so...\<close>
+
+datatype interp = Interp "observation" "(otxn \<Rightarrow> atxn)" "history"
+
+primrec history :: "interp \<Rightarrow> history" where
+"history (Interp obs m h) = h"
+
+text \<open>We say f is a total bijection between a and b iff f is bijective and every a maps to a b.
+I feel like there should be something for this in Isabelle already but I'm not sure.\<close>
+
+definition total_bij :: "('a \<Rightarrow> 'b) \<Rightarrow> 'a set \<Rightarrow> 'b set \<Rightarrow> bool" where
+"total_bij f as bs \<equiv> ((bij f) \<and> (\<forall>a. (a \<in> as) \<longrightarrow> ((f a) \<in> bs)))"
+
+(* I can't even show this? Really? *)
+lemma "(total_bij f as bs \<and> (b = (f a))) \<longrightarrow> (b \<in> bs)"
+  apply (simp add:total_bij_def)
+  apply auto
+  oops
+
+(* Huh, would have thought this would be easy *)
+lemma total_bij_image1: "(total_bij f a b) \<Longrightarrow> ((f`a) = b)"
+  apply (simp add: total_bij_def)
+
+  oops
+
+text \<open>Well-formed interpretations are made up of a well-formed observation, a bijection between
+observed and abstract transactions, and a well-formed history, such that the observation and 
+the history are compatible via that bijection.\<close>
+
+primrec wf_interpretation :: "interp \<Rightarrow> bool" where
+"wf_interpretation (Interp obs m h) = ((wf_observation obs) \<and>
+                                       (wf_history h) \<and>
+                                       (total_bij m (all_otxns obs) (all_atxns h)) \<and>
+                                       (is_compatible_observation obs m h))"
+
+text \<open>This lets us talk about corresponding transactions via that bijection m.\<close>
+
+primrec corresponding_atxn :: "interp \<Rightarrow> otxn \<Rightarrow> atxn" where
+"corresponding_atxn (Interp obs m h) otxn = (m otxn)"
+
+primrec corresponding_otxn :: "interp \<Rightarrow> atxn \<Rightarrow> otxn" where
+"corresponding_otxn (Interp obs m h) atxn = (THE otxn. atxn = m otxn)"
+
+text \<open>These are invertible, thanks to m being bijective.\<close>
+
+lemma "(corresponding_otxn (Interp obs h m) atxn) \<in> (all_otxns obs)"
+
+
+lemma corresponding_invertible: "(corresponding_otxn i (corresponding_atxn i t)) = t"
+  oops
+
+section \<open>Recoverability\<close>
+
+text \<open>Recoverability allows us to (in some cases) map a version of some key to a specific
+observed transaction which must have produced it. To start, we figure out when a transaction
+could have written a particular version of an object: some write resulting in this version of the
+object is compatible with a write in the transaction.\<close>
+
+definition could_have_been_written_by :: "object \<Rightarrow> version \<Rightarrow> otxn \<Rightarrow> bool" where
+"could_have_been_written_by obj v t \<equiv> (\<exists>aw ow. aw \<in> awrites_of obj v \<and>
+                                               ow \<in> all_owrites t \<and>
+                                               is_compatible_op ow aw)"
+
+(* might have this wrong *)
+lemma "((could_have_been_written_by obj v ot) \<and> (is_compatible_txn ot atxn)) \<longrightarrow>
+        (\<exists>v0 a r. (AWrite k v0 a v r) \<in> all_awrites atxn)"
+  oops
+
+
+text \<open>Given an observation, we say a version v of key k is recoverable to a transaction t if t is
+the only transaction which could have written that v of k.\<close>
+
+definition is_recoverable :: "observation \<Rightarrow> key \<Rightarrow> version \<Rightarrow> otxn \<Rightarrow> bool" where
+"is_recoverable obs k v ot \<equiv> (let obj = (THE ob. ob \<in> all_objects obs \<and> key ob = k) in
+                                (could_have_been_written_by obj v ot) \<and>
+                                (\<exists>!t. t \<in> all_otxns obs \<and> could_have_been_written_by obj v t))"
+
+
+
+
+end
