proof/Scratch.thy
@@ -1,0 +1,7 @@
+theory Scratch
+  imports Main Observation
+begin
+
+lemma "If a 
+
+end
